fix: redefine Euttc

CTree/Euttc.lean
@@ -1,50 +1,71 @@
-import CTree.Refinement
+import CTree.Basic
+import CTree.Monad
+import Mathlib.Data.ENat.Basic
 
 namespace CTree
-  /--
-  Equivalent up to tau and choice.
-  -/
-  def Euttc (r : Rel ρ σ) (t1 : CTree ε ρ) (t2 : CTree ε σ) : Prop :=
-    t1 ≤r≤ t2 ∧ t2 ≤flip r≤ t1
+  inductive EuttcF {ε : Type → Type} {ρ σ : Type}
+    (r : Rel ρ σ) (sim : ENat → ENat → CTree ε ρ → CTree ε σ → Prop)
+    : ENat → ENat → CTree ε ρ → CTree ε σ → Prop
+  | coind {p1 p2 t1 t2} (p1' p2' : ENat)
+      (h1 : p1' < p1) (h2 : p2' < p2) (h : sim p1' p2' t1 t2)
+      : EuttcF r sim p1 p2 t1 t2
+  | ret {x y p1 p2} (h : r x y) : EuttcF r sim p1 p2 (ret x) (ret y)
+  | vis {p1 p2} {α : Type} {e : ε α} {k1 : α → CTree ε ρ} {k2 : α → CTree ε σ}
+      (h : ∀ a : α, EuttcF r sim ⊤ ⊤ (k1 a) (k2 a)) : EuttcF r sim p1 p2 (vis e k1) (vis e k2)
+  | tau_left {p1 p2 t1 t2}
+      (h : EuttcF r sim ⊤ p2 t1 t2) : EuttcF r sim p1 p2 t1.tau t2
+  | tau_right {p1 p2 t1 t2}
+      (h : EuttcF r sim p1 ⊤ t1 t2) : EuttcF r sim p1 p2 t1 t2.tau
+  | zero {p1 p2} : EuttcF r sim p1 p2 zero zero
+  | choice_left {p1 p2 t1 t2 t3}
+      (h1 : EuttcF r sim ⊤ p2 t1 t3)
+      (h2 : EuttcF r sim ⊤ p2 t2 t3)
+      : EuttcF r sim p1 p2 (t1 ⊕ t2) t3
+  | choice_right {p1 p2 t1 t2 t3}
+      (h1 : EuttcF r sim p1 ⊤ t1 t2)
+      (h2 : EuttcF r sim p1 ⊤ t1 t3)
+      : EuttcF r sim p1 p2 t1 (t2 ⊕ t3)
+
+  theorem EuttcF.monotone (r : Rel ρ σ) (sim sim' : ENat → ENat → CTree ε ρ → CTree ε σ → Prop)
+    (hsim : ∀ p1 p2 t1 t2, sim p1 p2 t1 t2 → sim' p1 p2 t1 t2)
+    {p1 p2 t1 t2} (h : EuttcF r sim p1 p2 t1 t2) : EuttcF r sim' p1 p2 t1 t2 := by
+    induction h with
+    | coind _ _ h1 h2 h => exact .coind _ _ h1 h2 (hsim _ _ _ _ h)
+    | ret h => exact .ret h
+    | vis _ ih => exact .vis λ a => ih a
+    | tau_left _ ih => exact EuttcF.tau_left ih
+    | tau_right _ ih => exact EuttcF.tau_right ih
+    | zero => exact .zero
+    | choice_left _ _ ih1 ih2 => exact .choice_left ih1 ih2
+    | choice_right _ _ ih1 ih2 => exact .choice_right ih1 ih2
+
+  def Euttc' (r : Rel ρ σ) (p1 p2 : ENat) (t1 : CTree ε ρ) (t2 : CTree ε σ) : Prop :=
+    EuttcF r (Euttc' r) p1 p2 t1 t2
+    greatest_fixpoint monotonicity by
+      intro _ _ hsim _ _ _ _ h
+      apply EuttcF.monotone (hsim := hsim) (h := h)
+
+  abbrev Euttc (r : Rel ρ σ) (t1 : CTree ε ρ) (t2 : CTree ε σ) :=
+    ∃ p1 p2, Euttc' r p1 p2 t1 t2
 
   @[refl]
   theorem Euttc.refl {r : Rel ρ ρ} [IsRefl ρ r] : Euttc r t t :=
-    ⟨.refl _, .refl _⟩
+    sorry
 
   @[symm]
   theorem Euttc.symm {r : Rel ρ σ} (h : Euttc r t1 t2) : Euttc (flip r) t2 t1 :=
-    ⟨h.2, h.1⟩
+    sorry
 
   @[trans]
   theorem Euttc.trans (h1 : Euttc r1 t1 t2) (h2 : Euttc r2 t2 t3) : Euttc (r1.comp r2) t1 t3 :=
-    have heq : Rel.comp (flip r2) (flip r1) = flip (r1.comp r2) := by
-      funext x y
-      simp only [Rel.comp, flip, eq_iff_iff]
-      apply Iff.intro
-      · intro a
-        obtain ⟨w, h⟩ := a
-        obtain ⟨left, right⟩ := h
-        apply Exists.intro
-        · apply And.intro
-          on_goal 2 => {exact left
-          }
-          · simp_all only
-      · intro a
-        obtain ⟨w, h⟩ := a
-        obtain ⟨left, right⟩ := h
-        apply Exists.intro
-        · apply And.intro
-          on_goal 2 => {exact left
-          }
-          · simp_all only
-    ⟨.trans h1.1 h2.1, heq ▸ .trans h2.2 h1.2⟩
+    sorry
 
   instance : HasEquiv (CTree ε ρ) where
     Equiv := Euttc Eq
 
   @[refl]
   theorem Euttc.eq_refl {t : CTree ε ρ} : t ≈ t :=
-    ⟨.refl _, .refl _⟩
+    sorry
 
   @[symm]
   theorem Euttc.eq_symm {t1 t2 : CTree ε ρ} (h : t1 ≈ t2) : t2 ≈ t1 := by
@@ -65,65 +86,33 @@ namespace CTree
 
   namespace Euttc
     theorem choice_idemp (h1 : Euttc r t1 t3) (h2 : Euttc r t2 t3) : Euttc r (t1 ⊕ t2) t3 :=
-      ⟨.choice_idemp h1.1 h2.1, .choice_left h1.2⟩
+      sorry
 
     theorem choice_idemp_self {t : CTree ε ρ} : (t ⊕ t) ≈ t :=
       choice_idemp refl refl
 
     theorem choice_comm {t1 t2 : CTree ε ρ} : (t1 ⊕ t2) ≈ (t2 ⊕ t1) :=
-      ⟨
-        .choice_idemp (.choice_right <| .refl _) (.choice_left <| .refl _),
-        .choice_idemp (.choice_right <| .refl _) (.choice_left <| .refl _)
-      ⟩
+      sorry
 
     theorem zero_left_id (h : t1 ≈ t2) : (zero ⊕ t1) ≈ t2 :=
-      ⟨.choice_idemp .zero_le <| h.1, .choice_right <| h.2⟩
+      sorry
 
     theorem zero_right_id (h : t1 ≈ t2) : (t1 ⊕ zero) ≈ t2 :=
-      ⟨.choice_idemp h.1 .zero_le, .choice_left <| h.2⟩
+      sorry
 
     theorem choice_assoc {t1 t2 t3 : CTree ε ρ} : ((t1 ⊕ t2) ⊕ t3) ≈ (t1 ⊕ (t2 ⊕ t3)) :=
-      ⟨
-        .choice_idemp
-          (.choice_idemp (.choice_left <| .refl _) (.choice_right <| .choice_left <| .refl _))
-          (.choice_right <| .choice_right <| .refl _),
-        .choice_idemp
-          (.choice_left <| .choice_left <| .refl _)
-          (.choice_idemp (.choice_left <| .choice_right <| .refl _) (.choice_right <| .refl _))
-      ⟩
+      sorry
 
     theorem congr_map {t1 t2 : CTree ε ρ} {f : ρ → σ} (h : t1 ≈ t2) : t1.map f ≈ t2.map f :=
-      ⟨
-        .congr_map h.1,
-        by
-          have := Refine.congr_map (f := f) (flip_eq (r := Eq) ▸ h.2)
-          rw [flip_eq]
-          exact this
-      ⟩
+      sorry
 
     theorem map_trans {t1 t2 : CTree ε ρ} {t3 : CTree ε σ} {f : ρ → σ}
       (h1 : t1 ≈ t2) (h2 : t2.map f ≈ t3) : t1.map f ≈ t3 :=
-      .eq_trans h1.congr_map h2
+      sorry
 
     theorem vis_eq {e : ε α} {k1 k2 : α → CTree ε ρ}
       (h : ∀ a, k1 a ≈ k2 a) : vis e k1 ≈ vis e k2 :=
-      ⟨.vis λ a => (h a).left, .vis λ a => (h a).right⟩
-
-    def vis1 (e : ε α) : CTree ε ρ :=
-      vis e (λ _ => zero)
-
-    def vis2 (e1 e2 : ε α) : CTree ε ρ :=
-      vis e1 (λ _ => vis1 e2)
-
-    theorem choice_partial_vis_angelic : ((@vis1 ε ρ α e1) ⊕ (vis2 e1 e2)) ≈ vis2 e1 e2 := by
-      apply And.intro
-      · apply Refine.choice_idemp
-        · apply Refine.vis
-          intro a
-          exact Refine.zero_le
-        · exact Refine.refl _
-      · apply Refine.choice_right
-        exact Refine.refl _
+      sorry
 
   end Euttc
 
