CTree/LTS.lean
@@ -35,86 +35,9 @@ namespace CTree
   def IsWeakBisimulation (sim : Rel (CTree ε ρ) (CTree ε ρ)) : Prop :=
     IsWeakSimulation sim ∧ IsWeakSimulation (flip sim)
 
+  def WeakSim : Rel (CTree ε ρ) (CTree ε ρ) :=
+    λ p q => ∃ sim, IsWeakSimulation sim ∧ sim p q
+
   def WeakBisim : Rel (CTree ε ρ) (CTree ε ρ) :=
     λ p q => ∃ sim, IsWeakBisimulation sim ∧ sim p q
-
-  -- def vis1 (e : ε α) : CTree ε ρ :=
-  --   vis e (λ _ => zero)
-
-  -- def vis2 (e1 e2 : ε α) : CTree ε ρ :=
-  --   vis e1 (λ _ => vis1 e2)
-
-  -- theorem choice_partial_vis_angelic : WeakBisim ((@vis1 ε ρ α e1) ⊕ (vis2 e1 e2)) (vis2 e1 e2) := by
-  --   simp only [WeakBisim]
-  --   exists λ p q => p = (vis1 e1 ⊕ vis2 e1 e2) ∧ q = vis2 e1 e2
-  --   apply And.intro
-  --   · simp only [IsWeakBisimulation]
-  --     apply And.intro
-  --     · simp only [IsWeakSimulation]
-  --       intro p1 q1 ⟨heq1, heq2⟩ l p2' step
-  --       subst heq1 heq2
-  --       generalize hp : (vis1 e1 ⊕ vis2 e1 e2) = p at *
-  --       cases step
-  --       <;> ctree_elim hp
-  --       case choice_left h =>
-  --         have ⟨hl, hr⟩ := choice_inj hp
-  --         subst hl hr
-  --         generalize hv1 : vis1 e1 = v1 at *
-  --         cases h
-  --         <;> ctree_elim hv1
-  --         simp only
-  --         have hα := vis_inj_α hv1
-  --         subst hα
-  --         have ⟨he, hk⟩ := vis_inj hv1
-  --         subst he hk
-  --         exists vis1 e2
-  --         apply And.intro
-  --         · exists vis2 e1 e2, vis1 e2, 0, 0
-  --           apply And.intro
-  --           · simp only [NTauStep]
-  --           · apply And.intro
-  --             · simp only [vis2]
-  --               exact Step.vis (α := α) (e := e1) (k := fun _ => vis1 e2)
-  --             · simp only [NTauStep]
-  --         ·
-  --           sorry
-  --       case choice_right h =>
-  --         have ⟨hl, hr⟩ := choice_inj hp
-  --         subst hl hr
-  --         generalize hv2 : vis2 e1 e2 = v2 at *
-  --         cases h
-  --         <;> ctree_elim hv2
-  --         simp only
-  --         have hα := vis_inj_α hv2
-  --         subst hα
-  --         have ⟨he, hk⟩ := vis_inj hv2
-  --         subst he hk
-  --         exists vis1 e2
-  --         exists vis2 e1 e2, vis1 e2, 0, 0
-  --         apply And.intro
-  --         · simp only [NTauStep, vis2]
-  --         · apply And.intro
-  --           · simp only [vis2]
-  --             exact Step.vis (α := α) (e := e1) (k := fun _ => vis1 e2)
-  --           · simp only [NTauStep]
-  --     · simp only [IsWeakSimulation]
-  --       intro p1 q1 ⟨heq1, heq2⟩ l p2' step
-  --       subst heq1 heq2
-  --       generalize hp : vis2 e1 e2 = p at *
-  --       cases step
-  --       <;> ctree_elim hp
-  --       simp only
-  --       have hα := vis_inj_α hp
-  --       subst hα
-  --       have ⟨he, hk⟩ := vis_inj hp
-  --       subst he hk
-  --       exists vis1 e2
-  --       exists (vis1 e1 ⊕ vis e1 fun x => vis1 e2), vis1 e2, 0, 0
-  --       apply And.intro
-  --       · simp only [NTauStep]
-  --       · apply And.intro
-  --         · apply Step.choice_right
-  --           exact Step.vis
-  --         · simp only [NTauStep]
-  --   · simp_all only [and_self]
 end CTree
